\documentclass[a4paper,12pt]{article}\usepackage{amssymb,amsfonts,amsmath}\usepackage[english]{babel}\usepackage{latexsym}\usepackage{epsfig}% =======================================================================% Margins --- save forests\NeedsTeXFormat{LaTeX2e}\oddsidemargin -10 pt       %   Left margin on odd-numbered pages.\evensidemargin 10 pt       %   Left margin on even-numbered pages.\marginparwidth 1 in        %   Width of marginal notes.\oddsidemargin -1.5 true cm %   Note that \oddsidemargin = \evensidemargin\evensidemargin -1.5 true cm\marginparwidth 0.75 in\textwidth 7.5 true in % Width of text line.\textheight 26.0 true cm\topmargin -2.5 true cm% =======================================================================% Environments problem, solution, remark\newcount\probcnt\newenvironment{problem}[1]{%  \global\advance\probcnt1%  \goodbreak\medskip\par\noindent\textbf{Problem~\the\probcnt%    \if{#1}\empty\else~(#1)\fi.}~}%{%  \goodbreak}\newenvironment{solution}[1][]{%  \goodbreak\smallskip\par\noindent\textbf{Solution{\if#1\empty\else~#1\fi}.}~}%{%  \goodbreak}\newenvironment{remark}[1][]{  \goodbreak\smallskip\par  \small  \noindent\textbf{Remark{\if#1\empty\else~#1\fi}.}~%}{%  \goodbreak  \normalsize}\newenvironment{lemma}[1][]{  \goodbreak\smallskip\par  \noindent\textit{Lemma{\if#1\empty\else~#1\fi}.}~%}{%  \goodbreak\smallskip}\newenvironment{proof}[1][]{  \goodbreak\par  \noindent\textit{Proof{\if#1\empty\else~#1\fi}.}~%}{%  \goodbreak\smallskip}% =======================================================================%%% Some common macros\newcommand{\RR}{{\mathbb{R}}}\newcommand{\ZZ}{{\mathbb{Z}}}\newcommand{\CC}{{\mathbb{C}}}\newcommand{\QQ}{{\mathbb{Q}}}\newcommand{\NN}{{\mathbb{N}}}\newcommand{\tr}{\rm tr}\newcommand{\ds}{\displaystyle}\newcommand{\dx}{\mathrm{d}x}\newcommand{\dy}{\mathrm{d}y}\newcommand{\dz}{\mathrm{d}z}\newcommand{\dt}{\mathrm{d}t}\newcommand{\du}{\mathrm{d}u}\newcommand{\GL}{\operatorname{GL}}\newcommand{\rk}{\operatorname{rk}}% == TITLES ==========================================================\begin{document}\begin{center}  {\Large\textbf{Proposed problems for the IMC 2025}}\end{center}% =======================================================================%%% DOCUMENT_BEGIN% Do not change the document above this point% =======================================================================% =======================================================================% My macros% =======================================================================% Insert your macros here% \def\MyMacro{...}% =======================================================================\begin{problem}{Alex Avdiushenko, Neapolis University Paphos, Cyprus}  Find all strictly monotonic functions \(f:\mathbb{R}\to\mathbb{R}\) such that\[f(x)\,f^{-1}(x) = x^2.\]\end{problem}% -----------------------------------------------------------------------\begin{solution}  \begin{enumerate}    \item[\textbf{1.}] \textit{Value at the origin.}\;          Substituting \(x=0\) into equation gives          \[            f(0)\,f^{-1}(0)=0 .          \]          If \(f(0)\neq0\) then \(f^{-1}(0)=0\); applying \(f\) to both sides forces          \(f(0)=0\) --- a contradiction. Hence          \[            f(0)=0 \tag{1}          \]    \item[\textbf{2.}] It is clear that either there exists an \(a\) such that \(f(a)=ka\) with \(k\neq1\),    or else \(\forall x\, f(x)=x\).    Substituting \(x=ka\) into the given equation yields \( f(ka)=k^2a \).    Proceeding by induction, one easily shows that    \[      f\bigl(k^na\bigr)=k^{n+1}a      \qquad(n\in\mathbb{Z}_{\ge0}).    \]    Now take a number \(x\) lying between \(a\) and \(f(a) = ka\) and set \(f(x)=lx\).    By monotonicity, the value \(f^{n}(x)\) lies between \(f^{n}(a)\) and \(f^{n+1}(a)\).    In other words, the number \(l^{n}x\) is always situated between \(k^na\) and \(k^{n+1}a\),    whence it follows that \(l=k\).    \item[\textbf{3.}] Because \(f\) is a strictly monotonic bijection, every real          number lies between some (forward or backward) iterate of \(a\) and \(f(a) = ka\);    thus          \[            f(x) \equiv k\,x          \]    \item[\textbf{4.}] \textit{Verification.}\;          For \(f(x)=k\,x\) we have \(f^{-1}(x)=x/k\), hence          \[            f(x)\,f^{-1}(x)=\bigl(kx\bigr)\Bigl(\frac{x}{k}\Bigr)=x^{2}.          \]          If \(k>0\) the function is strictly increasing; if \(k<0\) it is          strictly decreasing, fulfilling the monotonicity requirement.  \end{enumerate}\end{solution}% =======================================================================\begin{problem}{Alex Avdiushenko, Neapolis University Paphos, Cyprus}  Find all continuous functions \(f:\mathbb{R}\to\mathbb{R}\) such that,  for every \(x,y\in\mathbb{R}\),  \[  (x-y)\,f(x+y) \;=\; (x+y)\,\bigl(f(x)-f(y)\bigr).  \]\end{problem}% -----------------------------------------------------------------------\begin{solution}\textbf{Answer:} \(ax^{2}+bx\).  \begin{enumerate}  \item \emph{$f(0)=0$.}  Put $y=0$ in the equation:        \[        x\,f(x)=x\bigl(f(x)-f(0)\bigr)\;\Longrightarrow\;f(0)=0.        \]  \item Consider the three special pairs $(1,z)$, $(1,z+1)$, $(2,z)$:  Fix $z\in\mathbb{R}\setminus\{0,1,2\}$.  Using original equation with the pairs listed, we successively get  \begin{align*}  (1,z):\;& f(1+z)=\frac{1+z}{1-z}\,f(1)-\frac{1+z}{1-z}\,f(z),\\[4pt]  (1,z+1):\;& f(z+2)=-\frac{2+z}{z}\,f(1)+\frac{2+z}{z}\,f(z+1),\\[4pt]  (2,z):\;& f(z+2)=\frac{2+z}{2-z}\,f(2)-\frac{2+z}{2-z}\,f(z).  \end{align*}  Substituting the first line into the second yields  \begin{align*}  f(z+2) = \frac{2+z}{z} \left(-f(1) + \frac{1+z}{1-z}\,f(1)-\frac{1+z}{1-z}\,f(z) \right) = \\[4pt]  = \frac{2+z}{z} \left(\frac{2z}{1-z}\,f(1)  - \frac{1+z}{1-z}\,f(z) \right) = \\[4pt]  = \frac{2(2+z)}{z(1-z)}\,f(1) - \frac{(2+z)(1+z)}{z(1-z)}\,f(z) \tag{3}  \end{align*}  \item Using the third line (for \((2, z)\)) and (3), we get  \begin{align*}  f(z+2) = \frac{2+z}{2-z}\,f(2)-\frac{2+z}{2-z}\,f(z) =  \frac{2(2+z)}{z(1-z)}\,f(1) - \frac{(2+z)(1+z)}{z(1-z)}\,f(z) \\[4pt]  \text{we reduce \((2+z)\)} \\[4pt]  \frac{1}{2-z}\,f(2)-\frac{1}{2-z}\,f(z) =  \frac{2}{z(1-z)}\,f(1) - \frac{1+z}{z(1-z)}\,f(z) \\[4pt]  \text{and group \(f(z)\)} \\[4pt]  \left( \frac{1+z}{z(1-z)} -\frac{1}{2-z} \right)\,f(z) =  \frac{2}{z(1-z)}\,f(1) - \frac{1}{2-z}\,f(2) \\[4pt]  \text{and multiply \(z(1-z)(2-z)\)} \\[4pt]  \left( (1+z)(2-z) - z(1-z) \right)\,f(z) = 2(2-z)\,f(1) - z(1-z)\,f(2) \\[4pt]  2 f(z) = 2(2-z)\,f(1) - z(1-z)\,f(2) \\[4pt]    f(z) = 2\,f(1) - z \left( f(1) + \frac{f(2)}{2} \right) + \frac{z^2}{2}\,f(2)  \end{align*}  \item That is, the function can only be quadratic, and \(f(0) = 0\),  and therefore \( f(x) = ax^2 + bx\), which, as can and should be verified,  satisfies the original equation.  \end{enumerate}  \remark{In a similar way it can be calculated that \(f(z+2) - 2f(z+1) + f(z) = 0\),  which is discrete analogue of ``second derivative = 0``.}\end{solution}\begin{problem}{Alex Avdiushenko, Neapolis University Paphos, Cyprus}Let $P,Q,R\in O(3)$ be real orthogonal $3\times 3$ matrices,i.e.\ $P^{\mathsf T}P=Q^{\mathsf T}Q=R^{\mathsf T}R=I_3$.Show that the matrix equation\[  P + Q \;=\; R\]has no solutions in $O(3)$.\end{problem}\begin{solution}Assume, for contradiction, that $P,Q,R\in O(3)$ satisfy $P+Q=R$.\smallskip\textbf{1.  Reduce to one orthogonal matrix.}Set\[S:=P^{\mathsf T}Q\in O(3),\qquadQ=PS,\qquadR=P(I_3+S).\]\textbf{2.  Orthogonality of $R$.}Because $R$ is orthogonal,\[I_3=R^{\mathsf T}R=(I_3+S)^{\mathsf T}(I_3+S)         =I_3+S^{\mathsf T}+S+S^{\mathsf T}S         =I_3+S^{\mathsf T}+S+I_3,\]whence\[S+S^{\mathsf T}=-I_3\]\textbf{3.  Minimal polynomial of $S$.}Multiplying the last identity on the left by $S$ gives\[S^2+S+I_3=0.\]Hence every eigenvalue $\lambda$ of $S$ satisfies $\lambda^2+\lambda+1=0$, i.e.\[\lambda=\exp\!\bigl(\pm 2\pi i/3\bigr)\quad(\text{non-real})\]\textbf{4.  Dimension parity contradiction.}For a real matrix, non-real eigenvalues occur in complex-conjugate pairs; thus a real $3\times3$ matrix with only non-real eigenvalues cannot exist (the dimension is odd).Therefore such an $S\in O(3)$ does not exist.\textbf{5.  Conclusion.}Since $S$ cannot exist, neither can a triple $(P,Q,R)\in O(3)^3$ with $P+Q=R$.Hence the equation admits \emph{no} solutions in $O(3)$.\remark{The same argument generalises to any dimension $n$.If an orthogonal matrix $S\in O(n)$ satisfies $S+S^{\mathsf T}=-I_n$, then it obeys the polynomial identity $S^{2}+S+I_n=0$; hence its eigenvalues are the two complex cubic roots of unity\[\lambda=\exp\!\bigl(\pm 2\pi i/3\bigr),\]which are non-real.Because complex eigenvalues of a real matrix occur in conjugate pairs, such an $S$ can exist only when the dimension $n$ is \emph{even}.Consequently, the $n=2$ construction based on a $120^\circ$ rotation extends to every even dimension by taking block-diagonal (direct sum) copies of the $2\times2$ block, whereas for every odd $n$ no orthogonal matrices $P,Q,R$ satisfy $P+Q=R$.}\end{solution}% =======================================================================% Do not change the document below this point%%% DOCUMENT_END% =======================================================================\end{document}